And update_last

dist/gcc-compatible/Hacl_Hash_SHA2.c
@@ -763,15 +763,139 @@ Hacl_Hash_SHA2_update_last_512(
   Hacl_Hash_SHA2_update_multi_512(s, tmp, tmp_len / (uint32_t)128U);
 }
 
-void
-(*Hacl_Hash_SHA2_hash_224)(uint8_t *x0, uint32_t x1, uint8_t *x2) = Hacl_Streaming_SHA2_sha224;
+void Hacl_Hash_SHA2_hash_224(uint8_t *input, uint32_t input_len, uint8_t *dst)
+{
+  uint32_t
+  s[8U] =
+    {
+      (uint32_t)0xc1059ed8U, (uint32_t)0x367cd507U, (uint32_t)0x3070dd17U, (uint32_t)0xf70e5939U,
+      (uint32_t)0xffc00b31U, (uint32_t)0x68581511U, (uint32_t)0x64f98fa7U, (uint32_t)0xbefa4fa4U
+    };
+  uint32_t blocks_n0 = input_len / (uint32_t)64U;
+  uint32_t blocks_n1;
+  if (input_len % (uint32_t)64U == (uint32_t)0U && blocks_n0 > (uint32_t)0U)
+  {
+    blocks_n1 = blocks_n0 - (uint32_t)1U;
+  }
+  else
+  {
+    blocks_n1 = blocks_n0;
+  }
+  uint32_t blocks_len0 = blocks_n1 * (uint32_t)64U;
+  uint8_t *blocks0 = input;
+  uint32_t rest_len0 = input_len - blocks_len0;
+  uint8_t *rest0 = input + blocks_len0;
+  uint32_t blocks_n = blocks_n1;
+  uint32_t blocks_len = blocks_len0;
+  uint8_t *blocks = blocks0;
+  uint32_t rest_len = rest_len0;
+  uint8_t *rest = rest0;
+  Hacl_Hash_SHA2_update_multi_224(s, blocks, blocks_n);
+  Hacl_Hash_SHA2_update_last_224(s, (uint64_t)blocks_len, rest, rest_len);
+  Hacl_Hash_Core_SHA2_finish_224(s, dst);
+}
 
-void
-(*Hacl_Hash_SHA2_hash_256)(uint8_t *x0, uint32_t x1, uint8_t *x2) = Hacl_Streaming_SHA2_sha256;
+void Hacl_Hash_SHA2_hash_256(uint8_t *input, uint32_t input_len, uint8_t *dst)
+{
+  uint32_t
+  s[8U] =
+    {
+      (uint32_t)0x6a09e667U, (uint32_t)0xbb67ae85U, (uint32_t)0x3c6ef372U, (uint32_t)0xa54ff53aU,
+      (uint32_t)0x510e527fU, (uint32_t)0x9b05688cU, (uint32_t)0x1f83d9abU, (uint32_t)0x5be0cd19U
+    };
+  uint32_t blocks_n0 = input_len / (uint32_t)64U;
+  uint32_t blocks_n1;
+  if (input_len % (uint32_t)64U == (uint32_t)0U && blocks_n0 > (uint32_t)0U)
+  {
+    blocks_n1 = blocks_n0 - (uint32_t)1U;
+  }
+  else
+  {
+    blocks_n1 = blocks_n0;
+  }
+  uint32_t blocks_len0 = blocks_n1 * (uint32_t)64U;
+  uint8_t *blocks0 = input;
+  uint32_t rest_len0 = input_len - blocks_len0;
+  uint8_t *rest0 = input + blocks_len0;
+  uint32_t blocks_n = blocks_n1;
+  uint32_t blocks_len = blocks_len0;
+  uint8_t *blocks = blocks0;
+  uint32_t rest_len = rest_len0;
+  uint8_t *rest = rest0;
+  Hacl_Hash_SHA2_update_multi_256(s, blocks, blocks_n);
+  Hacl_Hash_SHA2_update_last_256(s, (uint64_t)blocks_len, rest, rest_len);
+  Hacl_Hash_Core_SHA2_finish_256(s, dst);
+}
 
-void
-(*Hacl_Hash_SHA2_hash_384)(uint8_t *x0, uint32_t x1, uint8_t *x2) = Hacl_Streaming_SHA2_sha384;
+void Hacl_Hash_SHA2_hash_384(uint8_t *input, uint32_t input_len, uint8_t *dst)
+{
+  uint64_t
+  s[8U] =
+    {
+      (uint64_t)0xcbbb9d5dc1059ed8U, (uint64_t)0x629a292a367cd507U, (uint64_t)0x9159015a3070dd17U,
+      (uint64_t)0x152fecd8f70e5939U, (uint64_t)0x67332667ffc00b31U, (uint64_t)0x8eb44a8768581511U,
+      (uint64_t)0xdb0c2e0d64f98fa7U, (uint64_t)0x47b5481dbefa4fa4U
+    };
+  uint32_t blocks_n0 = input_len / (uint32_t)128U;
+  uint32_t blocks_n1;
+  if (input_len % (uint32_t)128U == (uint32_t)0U && blocks_n0 > (uint32_t)0U)
+  {
+    blocks_n1 = blocks_n0 - (uint32_t)1U;
+  }
+  else
+  {
+    blocks_n1 = blocks_n0;
+  }
+  uint32_t blocks_len0 = blocks_n1 * (uint32_t)128U;
+  uint8_t *blocks0 = input;
+  uint32_t rest_len0 = input_len - blocks_len0;
+  uint8_t *rest0 = input + blocks_len0;
+  uint32_t blocks_n = blocks_n1;
+  uint32_t blocks_len = blocks_len0;
+  uint8_t *blocks = blocks0;
+  uint32_t rest_len = rest_len0;
+  uint8_t *rest = rest0;
+  Hacl_Hash_SHA2_update_multi_384(s, blocks, blocks_n);
+  Hacl_Hash_SHA2_update_last_384(s,
+    FStar_UInt128_uint64_to_uint128((uint64_t)blocks_len),
+    rest,
+    rest_len);
+  Hacl_Hash_Core_SHA2_finish_384(s, dst);
+}
 
-void
-(*Hacl_Hash_SHA2_hash_512)(uint8_t *x0, uint32_t x1, uint8_t *x2) = Hacl_Streaming_SHA2_sha512;
+void Hacl_Hash_SHA2_hash_512(uint8_t *input, uint32_t input_len, uint8_t *dst)
+{
+  uint64_t
+  s[8U] =
+    {
+      (uint64_t)0x6a09e667f3bcc908U, (uint64_t)0xbb67ae8584caa73bU, (uint64_t)0x3c6ef372fe94f82bU,
+      (uint64_t)0xa54ff53a5f1d36f1U, (uint64_t)0x510e527fade682d1U, (uint64_t)0x9b05688c2b3e6c1fU,
+      (uint64_t)0x1f83d9abfb41bd6bU, (uint64_t)0x5be0cd19137e2179U
+    };
+  uint32_t blocks_n0 = input_len / (uint32_t)128U;
+  uint32_t blocks_n1;
+  if (input_len % (uint32_t)128U == (uint32_t)0U && blocks_n0 > (uint32_t)0U)
+  {
+    blocks_n1 = blocks_n0 - (uint32_t)1U;
+  }
+  else
+  {
+    blocks_n1 = blocks_n0;
+  }
+  uint32_t blocks_len0 = blocks_n1 * (uint32_t)128U;
+  uint8_t *blocks0 = input;
+  uint32_t rest_len0 = input_len - blocks_len0;
+  uint8_t *rest0 = input + blocks_len0;
+  uint32_t blocks_n = blocks_n1;
+  uint32_t blocks_len = blocks_len0;
+  uint8_t *blocks = blocks0;
+  uint32_t rest_len = rest_len0;
+  uint8_t *rest = rest0;
+  Hacl_Hash_SHA2_update_multi_512(s, blocks, blocks_n);
+  Hacl_Hash_SHA2_update_last_512(s,
+    FStar_UInt128_uint64_to_uint128((uint64_t)blocks_len),
+    rest,
+    rest_len);
+  Hacl_Hash_Core_SHA2_finish_512(s, dst);
+}
 
